StackLean/Dependent.lean
@@ -1,0 +1,191 @@
+import Mathlib.Order.Interval.Basic
+import Mathlib.Data.List.Nodup
+import Mathlib.Tactic
+import Init.Data.Vector.Basic
+import Aesop
+
+--- Basic Types ---
+
+abbrev Word := Fin (2 ^ 256)
+
+--- Sets ---
+
+-- We use a subtype here since it's more friendly to computable iteration than the mathlib sets
+def LSet (α : Type) := { l : List α // List.Nodup l }
+
+instance : Membership α (LSet α) where
+  mem (t : LSet α) (v : α) := v ∈ t.val
+
+instance (t : LSet α) (v : α) [DecidableEq α] : Decidable (v ∈ t) :=
+  inferInstanceAs (Decidable (v ∈ t.val))
+
+instance [DecidableEq α] : Sub (LSet α) where
+  sub (lhs : LSet α) (rhs : LSet α) : LSet α :=
+    ⟨lhs.val.filter (· ∉ rhs.val)
+    , by
+      apply List.Nodup.filter
+      exact lhs.property
+    ⟩
+
+def LSet.ofList [DecidableEq α] : (vs : List α) → LSet α
+  | .nil => ⟨[], by simp⟩
+  | .cons hd tl =>
+      let rest := LSet.ofList tl
+      if helem : hd ∈ rest
+      then rest
+      else
+      ⟨
+        hd :: rest.val,
+        by
+          simp ;
+          apply And.intro
+          · trivial
+          · apply rest.property
+      ⟩
+
+--- Stack Slots ---
+
+-- A var is a newtype around a Nat
+def Var := Nat
+  deriving DecidableEq
+
+-- In addition to variables, slots can contain literals and junk elems
+inductive Slot where
+  | Var : Var → Slot
+  | Lit : Word → Slot
+  | Junk : Slot
+  deriving DecidableEq
+
+instance : LawfulBEq Var := inferInstance
+instance : LawfulBEq Slot := inferInstance
+
+-- Stacks ---
+
+inductive Stack : List Slot → Type where
+  | Lit : (stk : List Slot) → Stack stk
+  | Push : Stack s → (lit: Word) → Stack ((.Lit lit) :: s)
+  | Pop : Stack (top :: rest) → Stack rest
+  | MarkJunk : Stack s → (ix : Fin s.length) → Stack (s.set ix .Junk)
+  | Swap1
+    : Stack (s00 :: s01 :: rest)
+    → Stack (s01 :: s00 :: rest)
+  | Swap2
+    : Stack (s00 :: s01 :: s02 :: rest)
+    → Stack (s02 :: s01 :: s00 :: rest)
+  | Swap3
+    : Stack (s00 :: s01 :: s02 :: s03 :: rest)
+    → Stack (s03 :: s01 :: s02 :: s00 :: rest)
+  | Swap4
+    : Stack (s00 :: s01 :: s02 :: s03 :: s04 :: rest)
+    → Stack (s04 :: s01 :: s02 :: s03 :: s00 :: rest)
+  | Swap5
+    : Stack (s00 :: s01 :: s02 :: s03 :: s04 :: s05 :: rest)
+    → Stack (s05 :: s01 :: s02 :: s03 :: s04 :: s00 :: rest)
+  | Swap6
+    : Stack (s00 :: s01 :: s02 :: s03 :: s04 :: s05 :: s06 :: rest)
+    → Stack (s06 :: s01 :: s02 :: s03 :: s04 :: s05 :: s00 :: rest)
+  | Swap7
+    : Stack (s00 :: s01 :: s02 :: s03 :: s04 :: s05 :: s06 :: s07 :: rest)
+    → Stack (s07 :: s01 :: s02 :: s03 :: s04 :: s05 :: s06 :: s00 :: rest)
+  | Swap8
+    : Stack (s00 :: s01 :: s02 :: s03 :: s04 :: s05 :: s06 :: s07 :: s08 :: rest)
+    → Stack (s08 :: s01 :: s02 :: s03 :: s04 :: s05 :: s06 :: s07 :: s00 :: rest)
+  | Swap9
+    : Stack (s00 :: s01 :: s02 :: s03 :: s04 :: s05 :: s06 :: s07 :: s08 :: s09 :: rest)
+    → Stack (s09 :: s01 :: s02 :: s03 :: s04 :: s05 :: s06 :: s07 :: s08 :: s00 :: rest)
+  | Swap10
+    : Stack (s00 :: s01 :: s02 :: s03 :: s04 :: s05 :: s06 :: s07 :: s08 :: s09 :: s10 :: rest)
+    → Stack (s10 :: s01 :: s02 :: s03 :: s04 :: s05 :: s06 :: s07 :: s08 :: s09 :: s00 :: rest)
+  | Swap11
+    : Stack (s00 :: s01 :: s02 :: s03 :: s04 :: s05 :: s06 :: s07 :: s08 :: s09 :: s10 :: s11 :: rest)
+    → Stack (s11 :: s01 :: s02 :: s03 :: s04 :: s05 :: s06 :: s07 :: s08 :: s09 :: s10 :: s00 :: rest)
+  | Swap12
+    : Stack (s00 :: s01 :: s02 :: s03 :: s04 :: s05 :: s06 :: s07 :: s08 :: s09 :: s10 :: s11 :: s12 :: rest)
+    → Stack (s12 :: s01 :: s02 :: s03 :: s04 :: s05 :: s06 :: s07 :: s08 :: s09 :: s10 :: s11 :: s00 :: rest)
+  | Swap13
+    : Stack (s00 :: s01 :: s02 :: s03 :: s04 :: s05 :: s06 :: s07 :: s08 :: s09 :: s10 :: s11 :: s12 :: s13 :: rest)
+    → Stack (s13 :: s01 :: s02 :: s03 :: s04 :: s05 :: s06 :: s07 :: s08 :: s09 :: s10 :: s11 :: s12 :: s00 :: rest)
+  | Swap14
+    : Stack (s00 :: s01 :: s02 :: s03 :: s04 :: s05 :: s06 :: s07 :: s08 :: s09 :: s10 :: s11 :: s12 :: s13 :: s14 :: rest)
+    → Stack (s14 :: s01 :: s02 :: s03 :: s04 :: s05 :: s06 :: s07 :: s08 :: s09 :: s10 :: s11 :: s12 :: s13 :: s00 :: rest)
+  | Swap15
+    : Stack (s00 :: s01 :: s02 :: s03 :: s04 :: s05 :: s06 :: s07 :: s08 :: s09 :: s10 :: s11 :: s12 :: s13 :: s14 :: s15 :: rest)
+    → Stack (s15 :: s01 :: s02 :: s03 :: s04 :: s05 :: s06 :: s07 :: s08 :: s09 :: s10 :: s11 :: s12 :: s13 :: s14 :: s00 :: rest)
+  | Swap16
+    : Stack (s00 :: s01 :: s02 :: s03 :: s04 :: s05 :: s06 :: s07 :: s08 :: s09 :: s10 :: s11 :: s12 :: s13 :: s14 :: s15 :: s16 :: rest)
+    → Stack (s16 :: s01 :: s02 :: s03 :: s04 :: s05 :: s06 :: s07 :: s08 :: s09 :: s10 :: s11 :: s12 :: s13 :: s14 :: s15 :: s00 :: rest)
+  | Dup1
+    : Stack (s00 :: rest)
+    → Stack (s00 :: s00 :: rest)
+  | Dup2
+    : Stack (s00 :: s01 :: rest)
+    → Stack (s01 :: s00 :: s01 :: rest)
+  | Dup3
+    : Stack (s00 :: s01 :: s02 :: rest)
+    → Stack (s02 :: s00 :: s01 :: s02 :: rest)
+  | Dup4
+    : Stack (s00 :: s01 :: s02 :: s03 :: rest)
+    → Stack (s03 :: s00 :: s01 :: s02 :: s03 :: rest)
+  | Dup5
+    : Stack (s00 :: s01 :: s02 :: s03 :: s04 :: rest)
+    → Stack (s04 :: s00 :: s01 :: s02 :: s03 :: s04 :: rest)
+  | Dup6
+    : Stack (s00 :: s01 :: s02 :: s03 :: s04 :: s05 :: rest)
+    → Stack (s05 :: s00 :: s01 :: s02 :: s03 :: s04 :: s05 :: rest)
+  | Dup7
+    : Stack (s00 :: s01 :: s02 :: s03 :: s04 :: s05 :: s06 :: rest)
+    → Stack (s06 :: s00 :: s01 :: s02 :: s03 :: s04 :: s05 :: s06 :: rest)
+  | Dup8
+    : Stack (s00 :: s01 :: s02 :: s03 :: s04 :: s05 :: s06 :: s07 :: rest)
+    → Stack (s07 :: s00 :: s01 :: s02 :: s03 :: s04 :: s05 :: s06 :: s07 :: rest)
+  | Dup9
+    : Stack (s00 :: s01 :: s02 :: s03 :: s04 :: s05 :: s06 :: s07 :: s08 :: rest)
+    → Stack (s08 :: s00 :: s01 :: s02 :: s03 :: s04 :: s05 :: s06 :: s07 :: s08 :: rest)
+  | Dup10
+    : Stack (s00 :: s01 :: s02 :: s03 :: s04 :: s05 :: s06 :: s07 :: s08 :: s09 :: rest)
+    → Stack (s09 :: s00 :: s01 :: s02 :: s03 :: s04 :: s05 :: s06 :: s07 :: s08 :: s09 :: rest)
+  | Dup11
+    : Stack (s00 :: s01 :: s02 :: s03 :: s04 :: s05 :: s06 :: s07 :: s08 :: s09 :: s10 :: rest)
+    → Stack (s10 :: s00 :: s01 :: s02 :: s03 :: s04 :: s05 :: s06 :: s07 :: s08 :: s09 :: s10 :: rest)
+  | Dup12
+    : Stack (s00 :: s01 :: s02 :: s03 :: s04 :: s05 :: s06 :: s07 :: s08 :: s09 :: s10 :: s11 :: rest)
+    → Stack (s11 :: s00 :: s01 :: s02 :: s03 :: s04 :: s05 :: s06 :: s07 :: s08 :: s09 :: s10 :: s11 :: rest)
+  | Dup13
+    : Stack (s00 :: s01 :: s02 :: s03 :: s04 :: s05 :: s06 :: s07 :: s08 :: s09 :: s10 :: s11 :: s12 :: rest)
+    → Stack (s12 :: s00 :: s01 :: s02 :: s03 :: s04 :: s05 :: s06 :: s07 :: s08 :: s09 :: s10 :: s11 :: s12 :: rest)
+  | Dup14
+    : Stack (s00 :: s01 :: s02 :: s03 :: s04 :: s05 :: s06 :: s07 :: s08 :: s09 :: s10 :: s11 :: s12 :: s13 :: rest)
+    → Stack (s13 :: s00 :: s01 :: s02 :: s03 :: s04 :: s05 :: s06 :: s07 :: s08 :: s09 :: s10 :: s11 :: s12 :: s13 :: rest)
+  | Dup15
+    : Stack (s00 :: s01 :: s02 :: s03 :: s04 :: s05 :: s06 :: s07 :: s08 :: s09 :: s10 :: s11 :: s12 :: s13 :: s14 :: rest)
+    → Stack (s14 :: s00 :: s01 :: s02 :: s03 :: s04 :: s05 :: s06 :: s07 :: s08 :: s09 :: s10 :: s11 :: s12 :: s13 :: s14 :: rest)
+  | Dup16
+    : Stack (s00 :: s01 :: s02 :: s03 :: s04 :: s05 :: s06 :: s07 :: s08 :: s09 :: s10 :: s11 :: s12 :: s13 :: s14 :: s15 :: rest)
+    → Stack (s15 :: s00 :: s01 :: s02 :: s03 :: s04 :: s05 :: s06 :: s07 :: s08 :: s09 :: s10 :: s11 :: s12 :: s13 :: s14 :: s15 :: rest)
+
+
+syntax "#Swap" num : term
+
+macro_rules
+  | `(#Swap $n:num) => return Lean.mkIdent (String.toName ((Lean.Name.toString `Stack.Swap).append (Nat.repr (Lean.TSyntax.getNat n))))
+
+
+abbrev FinIco (lo hi : Nat) := { val : Nat // lo ≤ val ∧ val < hi }
+
+syntax "#f" num : term
+
+macro_rules
+  | `(#f $n:num) => `(⟨$n, by omega⟩)
+
+inductive Stack' : Vector Slot sz → Type where
+  | Lit : (stk : Vector Slot sz) → Stack' stk
+  | Swap
+    : (idx : FinIco 1 (min 17 (.succ size)))
+    → Stack' (elems : Vector Slot (.succ size))
+    → (hlo : 0 < idx.val := by linarith)
+    → (htop : idx < elems.size := by linarith)
+    → Stack' (elems.swap 0 idx)
+
+def s' := Stack'.Lit #v[.Lit 0, .Lit 1]
+       |> (Stack'.Swap (#f 1))
+       --|> (Stack'.swap (#f 1))
